# x^2(y-x \frac{dy}{dx})=y(\frac{dy}{dx})^2

Column: Aug 27, 2020 3:19 PM
Last edited by: Soutrik das
Parent: Differential%20Equation%20140b16dfa0854772803fa71633eb3ff2.md
Tags: maths, question

This is a First order Second Degree Differential Equation and to solve it we need to [follow these steps](https://www.notion.so/Differential-Equation-140b16dfa0854772803fa71633eb3ff2#e97f655e28b74c92bab2801c9cb3523f) to break it into several first order First Degree Diff eq

$$x^2(y-x \frac{dy}{dx})=y(\frac{dy}{dx})^2 \tag{order=1 degree =2}$$

$$x^2y-x^3 \frac{dy}{dx}=y (\frac{dy}{dx})^2$$

Putting $p=\frac{dy}{dx}$

$$x^2y-x^3p=yp^2$$

Now time to break it like a quadratic ( ie Middle Term Factorization) but its not breaking

$$yp^2+x^3p-x^2y=0$$

$$p=\frac{-x^3 \pm \sqrt{x^6+4y^2x^2}}{2y}$$